import Relation.Binary.PropositionalEquality as Eq
open Eq using (_â‰¡_; refl; sym; trans; cong)
open import Data.Nat using (â„•; zero; suc; _+_; _*_; _âˆ¸_; _â‰¤_; _<_ ; sâ‰¤s; zâ‰¤n ; â‰¤-pred)
open import Data.Product

data Singleton {a} {A : Set a} (x : A) : Set a where
  _withâ‰¡_ : (y : A) â†’ x â‰¡ y â†’ Singleton x

inspect : âˆ€ {a} {A : Set a} (x : A) â†’ Singleton x
inspect x = x withâ‰¡ refl

const : â„• â†’ â„• â†’ â„•
const n _ = n

id : âˆ€ {â„“} {A : Set â„“} â†’ A â†’ A
id a = a



-- Dems
+0 : âˆ€ (x : â„•) â†’ x + 0 â‰¡ x
+0 zero = refl
+0 (suc x) rewrite +0 x = refl

<-pred : âˆ€ { n m : â„• } â†’ (suc n) < (suc m) â†’ n < m
<-pred = â‰¤-pred 


<â‡’â‰¤ : âˆ€ {n m : â„•} â†’ n < m â†’ n â‰¤ m
<â‡’â‰¤ {0} {m} p = zâ‰¤n
<â‡’â‰¤ {suc n} {0} ()
<â‡’â‰¤ {suc n} {suc m} p = sâ‰¤s (<â‡’â‰¤ {n} {m} (<-pred p)) 


â‰¤-trans : âˆ€ {a b c : â„•} â†’ a â‰¤ b â†’ b â‰¤ c â†’ a â‰¤ c
â‰¤-trans {0} {b} {c} p q = zâ‰¤n
â‰¤-trans {(suc n)} {0} {_} ()
â‰¤-trans {_} {(suc n)} {0} _ ()
â‰¤-trans {(suc m)} {(suc n)} {(suc t)} p q = sâ‰¤s (â‰¤-trans {m} {n} {t} (â‰¤-pred p) (â‰¤-pred q))

data ð”¹ : Set where
    tt : ð”¹
    ff : ð”¹


eq : â„• â†’ â„• â†’ ð”¹
eq 0 0 = tt
eq 0 (suc n) = ff
eq (suc n) 0 = ff
eq (suc m) (suc n) = eq n m

lt : â„• â†’ â„• â†’ ð”¹
lt _ 0 = ff
lt 0 (suc n) = tt
lt (suc n) (suc m) = lt n m

le : â„• â†’ â„• â†’ ð”¹
le 0 m = tt
le (suc n) 0 = ff
le (suc n) (suc m) = le n m

ð”¹-contra : (ff â‰¡ tt) â†’ âˆ€ {P : Set} â†’ P 
ð”¹-contra ()

sum : (â„• â†’ â„•) â†’ (i : â„•) â†’ (j : â„•) â†’ â„•
sum f n m with (eq n m)
sum f n m | tt  = f n
sum f n m | ff with inspect (lt n m)
sum f n m | ff | ff withâ‰¡ _ = 0 
sum f n (suc m) | ff | tt withâ‰¡ p = sum f n m + f (suc m) 
sum f n 0 | ff | tt withâ‰¡ n<0 = ð”¹-contra n<0

suc-inj : âˆ€ (a b : â„•) â†’ suc a â‰¡ suc b â†’ a â‰¡ b
suc-inj _ _ refl = refl

+l-elim : âˆ€ (a b c : â„•) â†’ a + b â‰¡ a + c â†’ b â‰¡ c
+l-elim 0 _ _ p = p
+l-elim (suc n) b c p = +l-elim n b c (suc-inj (n + b) (n + c) p) 

le-suc : âˆ€ {n m : â„•} â†’ (le n m â‰¡ tt) â†’ (le (suc n) (suc m) â‰¡ tt)
le-suc {0} {0} p = refl
le-suc {suc n} {0} ()
le-suc {m} {n} p = p

le-rsuc : âˆ€ {n m : â„•} â†’ (le n m â‰¡ tt) â†’ (le n (suc m) â‰¡ tt)
le-rsuc {0} {0} p = refl
le-rsuc {suc n} {0} ()
le-rsuc {0} {_} p = refl
le-rsuc {suc n} {suc m} p = le-rsuc {n} {m} p

lt-suc : âˆ€ {n m : â„•} â†’ (lt n m â‰¡ tt) â†’ (lt (suc n) (suc m) â‰¡ tt)
lt-suc {0} {0} ()
lt-suc {suc n} {0} ()
lt-suc {m} {n} p = p

lt-rsuc : âˆ€ {n m : â„•} â†’ (lt n m â‰¡ tt) â†’ (lt n (suc m) â‰¡ tt)
lt-rsuc {0} {0} p = refl
lt-rsuc {suc n} {0} ()
lt-rsuc {0} {_} p = refl
lt-rsuc {suc n} {suc m} p = lt-rsuc {n} {m} p

eq-sym : âˆ€ (m n : â„•) â†’ (eq n m) â‰¡ (eq m n)
eq-sym 0 0 = refl 
eq-sym 0 (suc n) = refl
eq-sym (suc n) 0 = refl
eq-sym (suc n) (suc m) = eq-sym m n

eq-suc : âˆ€ (m n : â„•) â†’ eq n m â‰¡ eq (suc n) (suc m)
eq-suc 0 0 = refl 
eq-suc 0 (suc n) = refl
eq-suc (suc n) 0 = refl
eq-suc (suc n) (suc m) = eq-suc m n

sum-last-term : âˆ€ ( f : â„• â†’ â„• ) (n m : â„•) â†’ le n m â‰¡ tt â†’ sum f n (suc m) â‰¡ sum f n m + f (suc m)
sum-last-term f n m p = {!!}



<-is-lt : âˆ€ {n m : â„•} â†’ n < m â†’ lt n m â‰¡ tt
<-is-lt {0} {0} ()
<-is-lt {_} {0} ()
<-is-lt {0} {suc m} p = refl
<-is-lt {suc n} {suc m} p = <-is-lt (<-pred p)


sum-assoc-from-0 : âˆ€ (f : â„• â†’ â„•) (j k : â„•)
                 â†’ (le j k â‰¡ tt)
                 â†’ (sum f 0 j) + sum f (suc j) k â‰¡ sum f 0 k
sum-assoc-from-0 f 0 k p = {!!} 
sum-assoc-from-0 = {!!}


1-le-suc : âˆ€ (n : â„•) â†’ le 1 (suc n) â‰¡ tt
1-le-suc 0 = refl
1-le-suc (suc n) = refl

sum-safe : (â„• â†’ â„•) â†’ (i : â„•) â†’ (j : â„•) â†’ (le i j â‰¡ tt) â†’ â„•
sum-safe f 0 0 p = f 0
sum-safe f (suc n) 0 ()
sum-safe f 0 (suc m) p = (sum-safe f 0 m refl) + f (suc m)
sum-safe f (suc n) (suc m) p = {!f (suc m) + !}



~_ : ð”¹ â†’ ð”¹
~ tt = ff
~ ff = tt

~~-elim : âˆ€ (b : ð”¹) â†’ ~ ~ b â‰¡ b
~~-elim tt = refl
~~-elim ff = refl


